map/MapMAproof.v
@@ -1,89 +1,74 @@
 Require Import CRIS.
-
-From CRIS.map Require Import Header MapM MapA.
-
-Set Implicit Arguments.
-
-Local Open Scope nat_scope.
+Require Export MapHeader MapM MapA.
 
 Module MapMA. Section MapMA.
-  Import MapAS.
-  Context `{!crisG Γ Σ α β τ _S _I}.
-  Context `{!mapMG}.
-  Context `{!mapG}.
+  Context `{!crisG Γ Σ α β τ _S _I, !concGS, !mapMGS, !mapGS}.
+  Import MapA.
 
-  Context (sp_s sp_t : sp_type).
-  Context (MapInSpS : sp_incl MapAS.sp sp_s).
-  Context (MapInSpT : sp_incl MapMS.sp sp_t).
+  Context (sp_s sp_t : specmap).
+  Context (MapInSpS : MapA.sp ⊆ sp_s).
+  Context (MapInSpT : MapM.sp ⊆ sp_t).
 
-
-  Definition Ist : alist key Any.t → alist key Any.t → iProp Σ :=
+  Definition Ist : ist_type Σ :=
     (λ st_src st_tgt,
       ∃ f sz,
-        ⌜st_src = [(MapA.v_map, f↑)] ∧ st_tgt = [(MapM.v_size, sz↑); (MapM.v_map, f↑)]⌝
-        ∗ (⌜f = (λ _ : Z, 0%Z) ∧ sz = 0%Z⌝
-            ∗ MapMS.pending
-            ∗ initial_map
-          ∨ pending
-            ∗ auth_allocated f
-            ∗ auth_unallocated sz))%I.
+        ⌜st_src = {[MapA.v_map := Some f↑]} ∧
+        st_tgt = {[MapM.v_size := Some sz↑; MapM.v_map := Some f↑]}⌝ ∗
+        (⌜f = (λ _ : Z, 0%Z) ∧ sz = 0%Z⌝ ∗ MapM.pending ∗ initial_map ∨
+          pending ∗ auth_allocated f ∗ auth_unallocated sz))%I.
 
   Local Definition MapA := (MapA.t sp_s).
   Local Definition MapM := (MapM.t sp_t).
 
-  Lemma simF_init : ISim.sim_fun open MapA MapM MapA.init_cond Ist (Some MapHdr.init).
+  Lemma simF_init : ISim.sim_fun open MapA MapM Ist (Some MapHdr.init).
   Proof using MapInSpS MapInSpT.
-    init_simF.
+    iStartSim.
 
-    steps_l.
-    iDestruct "ASM" as "[-> [[-> %range] P]]".
+    steps_l. rename _q into sz. iDestruct "ASM" as "[-> [[-> %range] P]]".
 
     (* SRC: handle the IST of Map and the precond of init *)
-    iDestruct "IST" as (f sz) "(% & [(% & P0 & INIT) | (P' & B & U)])"; cycle 1.
+    iDestruct "IST" as (f ?) "(% & [(% & P0 & INIT) | (P' & B & U)])"; cycle 1.
     { iExFalso. iApply (pending_unique with "P P'"). }
-    des. hss. rename _q into sz.
+    des; subst.
     
     (* TGT: prove the precond of init *)
-    step_r. force_r sz. force_r ([Vint sz] ↑). force_r.
-    iSplitL "P0". { iFrame. eauto. }
+    force_r sz. force_r ([Vint sz] ↑). force_r.
+    iSplitL "P0"; [iFrame; eauto|].
 
     (* TGT: handle the postcond of init *)
-    hss. steps_r. iDestruct "GRT" as "(% & %)". hss.
+    steps_r. iDestruct "GRT" as "(% & %)". subst.
     
     (* SRC: prove the postcond of init *)
     iMod (initialize with "INIT") as "(ALLOC & UNALLOC & INIT)".
     force_l. steps_l. force_l. force_l.
-    iSplitL "INIT". { iFrame. eauto. }
+    iSplitL "INIT"; [iFrame; eauto|].
     
     (* prove the IST of Map *)
     step. iSplit; eauto.
     iExists _, _. iSplitR; eauto. iRight. iFrame.
   (*SLOW*)Qed.
 
-  Lemma simF_get : ISim.sim_fun open MapA MapM MapA.init_cond Ist (Some MapHdr.get).
+  Lemma simF_get : ISim.sim_fun open MapA MapM Ist (Some MapHdr.get).
   Proof using MapInSpS MapInSpT.
-    init_simF.
+    iStartSim.
 
-    steps_l.
-    iDestruct "ASM" as "(-> & (-> & MAP))".
-    rename _q1 into k.
+    steps_l. destruct _q as [idx v]. iDestruct "ASM" as "(-> & (-> & MAP))".
 
     (* SRC: handle the IST of Map and the precond of get *)
     iDestruct "IST" as (f sz) "(% & [(% & P0 & INIT)|(P' & B & U)])".
     { iExFalso. iApply (initial_map_points_to with "INIT MAP"). }
-    hss. steps_l. hss. steps_l.
+    des; subst. steps_l.
 
     (* TGT: prove the precond of get *)
-    step_r. force_r k. force_r. force_r.
+    force_r idx. force_r. force_r.
     iSplit; first eauto.
 
     (* TGT : handle the body of get *)
-    hss. steps_r. hss. steps_r.
     iPoseProof (auth_unallocated_points_to with "U MAP") as "%".
-    force_r; iSplit; first eauto.
+    steps_r. rewrite /assume; unshelve force_r; eauto.
 
     (* TGT: handle the postcond of get *)
-    steps_r. hss. steps_r. iDestruct "GRT" as "(<- & _)".
+    steps_r. iDestruct "GRT" as "(<- & _)".
 
     (* SRC: prove the postcond of get *)
     force_l. force_l.
@@ -95,9 +80,9 @@ Module MapMA. Section MapMA.
     iExists _, _. iSplit; eauto. iRight. iFrame.
   (*SLOW*)Qed.
 
-  Lemma simF_set : ISim.sim_fun open MapA MapM MapA.init_cond Ist (Some MapHdr.set).
+  Lemma simF_set : ISim.sim_fun open MapA MapM Ist (Some MapHdr.set).
   Proof using MapInSpS MapInSpT.
-    init_simF.
+    iStartSim.
 
     (* SRC: handle the IST of Map and the precond of set *)
     do 2 step_l.
@@ -105,15 +90,15 @@ Module MapMA. Section MapMA.
     iDestruct "ASM" as "(-> & (-> & MAP))".
     iDestruct "IST" as (f sz) "(% & [(% & P0 & INIT)|(P' & B & U)])".
     { iExFalso. iApply (initial_map_points_to with "INIT MAP"). }
-    des. hss. steps_l. hss. steps_l. hss.
+    des; subst. steps_l.
 
     (* TGT: prove the precond of set *)
-    step_r. force_r (k, v). force_r. force_r. iSplitR; first eauto.
+    force_r (k, v). force_r. force_r. iSplitR; first eauto.
 
     (* TGT : handle the body of set *)
-    hss. steps_r. hss. steps_r.
+    steps_r. rewrite /assume.
     iPoseProof (auth_unallocated_points_to with "U MAP") as "%".
-    force_r; iSplit; first done. steps_r. hss. steps_r.
+    unshelve force_r; eauto. steps_r.
 
     (* TGT: handle the postcond of set *)
     iDestruct "GRT" as "(<- & _)".
@@ -127,67 +112,58 @@ Module MapMA. Section MapMA.
     iExists _, _. iSplit; eauto. iRight. iFrame.
   (*SLOW*)Qed.
 
-  Lemma simF_set_by_user : ISim.sim_fun open MapA MapM MapA.init_cond Ist (Some MapHdr.set_by_user).
+  Lemma simF_set_by_user : ISim.sim_fun open MapA MapM Ist (Some MapHdr.set_by_user).
   Proof using MapInSpS MapInSpT.
-    init_simF.
+    iStartSim.
 
     (* SRC: handle the IST of Map and the precond of set_by_user *)
     do 2 step_l. destruct _q as [k w]. steps_l.
-    iDestruct "ASM" as "(-> & (-> & MAP))".
-    hss. steps_l.
+    iDestruct "ASM" as "(-> & (-> & MAP))". steps_l.
 
     (* TGT: prove the precond of set_by_user *)
-    step_r. force_r. force_r. force_r. hss. iSplitR. { eauto. }
+    force_r. force_r. force_r. iSplitR. { eauto. }
 
     (* process an input *)
     steps_r. step.
 
     (* TGT: handle the precond of set *)
-    steps_r. iDestruct "GRT" as "%". des. hss.
+    steps_r. simpl_sp. steps_r. destruct _q as [? ?]; iDestruct "GRT" as "%". des; hss.
     
     (* SRC: prove the precond of set *)
-    steps_l. force_l (_,_,_). force_l. force_l.
+    steps_l. simpl_sp. force_l (_,_,_). force_l. force_l.
     iSplitL "MAP". { iFrame. eauto. }
 
     (* make a call to set *)
     call "IST".
 
     (* SRC: handle the postcond of set *)
-    steps_l. iDestruct "ASM" as "(-> & (-> & MAP))". hss.
+    clear_st; iIntros (ret st_src st_tgt) "IST".
+    steps_l. iDestruct "ASM" as "(-> & (-> & MAP))". steps_l; steps_r.
 
     (* TGT: prove the postcond of set *)
-    steps_l. force_r. force_r. iSplitR. { iFrame. eauto. }
+    force_r. force_r. iSplitR. { iFrame. eauto. }
 
     (* TGT: handle the postcond of set_by_user *)
-    steps_r. hss. steps_r. iDestruct "GRT" as "(<- & _)".
+    steps_r. iDestruct "GRT" as "(<- & _)".
     
     (* SRC: prove the postcond of set_by_user *)
     force_l. force_l. iSplitL "MAP". { iFrame. eauto. }
 
     (* prove the IST of Map *)
-    step. eauto.
+    step. iFrame. eauto.
   (*SLOW*)Qed.
 
   Lemma sim : ISim.t open MapA MapM MapA.init_cond Ist.
   Proof using MapInSpS MapInSpT.
     init_sim.
-    - split; eauto. iIntros "(IST & P)"; s. iModIntro.
-      iExists _, _. iSplit; eauto. iLeft. iFrame. eauto.
-    - apply simF_init; eauto.
-    - apply simF_get; eauto.
-    - apply simF_set; eauto.
-    - apply simF_set_by_user; eauto.
+    { iIntros "(IST & P)"; s. iExists _, _. iSplit; eauto. iLeft. iFrame. eauto. }
+    { apply simF_init; eauto. }
+    { apply simF_get; eauto. }
+    { apply simF_set; eauto. }
+    { apply simF_set_by_user; eauto. }
   Qed.
-End MapMA.
 
-Section MapMA.
-  Context `{!crisG Γ Σ α β τ _S _I}.
-  Context `{!mapMG}.
-  Context `{!mapG}.
-
-  Lemma ctxr sp_s sp_t
-      (MapInSpS : sp_incl MapAS.sp sp_s)
-      (MapInSpT : sp_incl MapMS.sp sp_t) :
+  Lemma ctxr :
     ctx_refines
       (MapA.t sp_s, MapA.init_cond)
       (MapM.t sp_t, emp%I).
