map/MapHeader.v
@@ -1,0 +1,9 @@
+Require Import CRIS.
+Require Export ImpPrelude.
+
+Module MapHdr.
+  Definition init := "Map.init".
+  Definition get  := "Map.get".
+  Definition set  := "Map.set".
+  Definition set_by_user := "Map.set_by_user".
+End MapHdr.
