map/MapIAproof.v
@@ -1,27 +1,18 @@
 Require Import CRIS MemA.
-
-From CRIS.map Require Import Header MapA MapM MapI MapIMproof MapMAproof.
+Require Export MapHeader MapA MapM MapI MapIMproof MapMAproof.
 
 Module MapIA. Section MapIA.
-  Context `{!crisG Γ Σ α β τ _S _I}.
-  Context `{!mapMG}.
-  Context `{!mapG}.
-  Context `{!memG}.
+  Context `{!crisG Γ Σ α β τ _S _I, !concGS, !mapMGS, !mapGS, !memGS}.
 
-  Lemma ctxr (sp_s : sp_type)
-      (MapInSpMap : sp_incl MapAS.sp sp_s) :
+  Lemma ctxr (sp_s sp_mem : specmap)
+      (MapInSpMap : MapA.sp ⊆ sp_s) :
     ctx_refines
-      ((MapA.t sp_s) ★ (MemA.t), (MapA.init_cond ∗ MapM.init_cond)%I)
-      ((MapI.t)      ★ (MemA.t), emp%I).
+      (MapA.t sp_s ★ MemA.t sp_mem, MapA.init_cond)
+      (MapI.t      ★ MemA.t sp_mem, emp%I).
   Proof.
     etrans; cycle 1.
-    { eapply MapIM.ctxr.
-      instantiate (1:= to_sp MapMS.sp).
-      i. split; try refl. unfold MapMS.sp. unseal CRIS. prove_nodup.
-      i. unfold to_sp, MapMS.sp in *; rewrite H2; ss.
-    }
-    eapply ctxr_frameR. rewrite (mod_addc_empty_l (MapM.t _)). eapply ctxr_cond_frameR.
-    eapply MapMA.ctxr; eauto. unfold MapMS.sp. unseal CRIS. prove_nodup.
-    i. unfold to_sp, MapMS.sp in *; rewrite H2; ss.
+    { eapply MapIM.ctxr. instantiate (1:= MapM.sp); refl. }
+    eapply ctxr_frameR.
+    eapply MapMA.ctxr; eauto.
   Qed.
 End MapIA. End MapIA.
